pcuic/theories/PCUICEtaExpand.v
@@ -3,6 +3,9 @@ From MetaCoq.PCUIC Require Import PCUICAst PCUICAstUtils PCUICTyping.
 Definition isConstruct t :=
    match t with tConstruct _ _ _ => true | _ => false end.
 
+ Definition isFix t :=
+  match t with tFix _ _ => true | _ => false end.
+
 Section expanded.
 
 Variable Σ : global_env.
@@ -23,7 +26,13 @@ Inductive expanded : term -> Prop :=
 | expanded_tCase (ci : case_info) (type_info:predicate term)
         (discr:term) (branches : list (branch term)) : expanded discr -> Forall (fun br => expanded br.(bbody)) branches -> expanded (tCase ci type_info discr branches)
 | expanded_tProj (proj : projection) (t : term) : expanded t -> expanded (tProj proj t)
-| expanded_tFix (mfix : mfixpoint term) (idx : nat) :   Forall (fun d => expanded d.(dtype) /\ expanded d.(dbody)) mfix -> expanded (tFix mfix idx)
+| expanded_tFix (mfix : mfixpoint term) (idx : nat) args d : 
+  Forall (fun d => expanded d.(dtype) /\ expanded d.(dbody)) mfix ->
+  Forall expanded args ->
+  args <> [] ->
+  nth_error mfix idx = Some d ->
+  #|args| > d.(rarg) ->
+  expanded (mkApps (tFix mfix idx) args)
 | expanded_tCoFix (mfix : mfixpoint term) (idx : nat) :   Forall (fun d => expanded d.(dtype) /\ expanded d.(dbody)) mfix -> expanded (tCoFix mfix idx)
 | expanded_tConstruct_app ind c u mind idecl cdecl args :
     declared_constructor Σ (ind, c) mind idecl cdecl ->
@@ -60,13 +69,19 @@ forall (Σ : global_env) (P : term -> Prop),
  Forall (fun br : branch term => expanded Σ (bbody br)) branches ->
  Forall (fun br : branch term => P (bbody br)) branches ->
  P (tCase ci type_info discr branches)) ->
-(forall (proj : projection) (t : term),
- expanded Σ t -> P t -> P (tProj proj t)) ->
-
- (forall (mfix : mfixpoint term) (idx : nat), 
+ (forall (proj : projection) (t : term),
+ expanded Σ t -> P t -> P (tProj proj t)) -> 
+ (forall (mfix : mfixpoint term) (idx : nat) d args, 
  Forall (fun d => expanded Σ d.(dtype) /\ expanded Σ d.(dbody)) mfix -> 
  Forall (fun d => P d.(dtype) /\ P d.(dbody)) mfix -> 
- P (tFix mfix idx)) ->
+ Forall (expanded Σ) args ->
+ Forall P args ->
+ args <> [] ->
+ nth_error mfix idx = Some d ->
+ #|args| > d.(rarg) ->
+ expanded Σ (mkApps (tFix mfix idx) args) ->
+ P (mkApps (tFix mfix idx) args)) ->
+ 
 (forall (mfix : mfixpoint term) (idx : nat), 
  Forall (fun d => expanded Σ d.(dtype) /\ expanded Σ d.(dbody)) mfix -> 
  Forall (fun d => P d.(dtype) /\ P d.(dbody)) mfix -> 
@@ -88,7 +103,7 @@ Proof.
   - assert (Forall P args) by (induction H15; econstructor; eauto).
     destruct f0; eauto.
   - eapply H9; eauto. induction H14; econstructor; eauto.
-  - eapply H11; eauto. induction H14 as [ | ? ? []]; econstructor; cbn in *; eauto; split.
+  - eapply H11; eauto. 3: eapply expanded_tFix; eauto. clear -H14 f. induction H14; econstructor; firstorder. clear - H15 f. induction H15; econstructor; firstorder.
   - eapply H12; eauto. induction H14 as [ | ? ? []]; econstructor; cbn in *; eauto; split.
   - eapply H13; eauto. clear - f H16. induction H16; econstructor; cbn in *; eauto; split.
 Qed.
