pcuic/theories/PCUICWcbvEval.v
@@ -2,9 +2,8 @@
 From Coq Require Import CRelationClasses.
 From MetaCoq.Template Require Import config utils.
 From MetaCoq.PCUIC Require Import PCUICAst PCUICAstUtils PCUICLiftSubst
-     PCUICUnivSubst PCUICTyping PCUICGlobalEnv PCUICReduction PCUICClosed 
-     PCUICClosedTyp PCUICCSubst 
-     PCUICSubstitution PCUICInversion.
+     PCUICUnivSubst PCUICTyping PCUICGlobalEnv PCUICReduction PCUICClosed PCUICCSubst
+     PCUICClosedTyp. (* Due to reliance on wf Σ instead of closed_env Σ *)
 
 Require Import ssreflect ssrbool.
 From Equations Require Import Equations.
